

Introduction to general relativity: the Schwarzschild solution

28 June 2021 10:19

$$ds^2 = -f(r) dt^2 + h(r) dr^2 + r^2 (d\theta^2 + \sin^2\theta d\phi^2)$$

we need to solve for these

The nonzero components of metric

$$g_{tt} = -f(r) ; \quad g_{rr} = h(r) ; \quad g_{\theta\theta} = r^2 ; \quad g_{\phi\phi} = r^2 \sin^2\theta$$

Inverse

$$g^{tt} = -f^{-1}(r) ; \quad g^{rr} = h^{-1}(r) ; \quad g^{\theta\theta} = r^{-2} ; \quad g^{\phi\phi} = r^{-2} \sin^{-2}\theta$$

Christoffel symbols

$$\Gamma_{\mu\nu}^{\lambda} = \frac{1}{2} g^{\lambda\rho} \left(\frac{\partial g_{\rho\mu}}{\partial x^{\nu}} + \frac{\partial g_{\rho\nu}}{\partial x^{\mu}} - \frac{\partial g_{\mu\nu}}{\partial x^{\rho}} \right)$$

Show (ex).

$$\begin{aligned} \Gamma_{rr}^r &= \frac{1}{2h(r)} \frac{dh(r)}{dr}, & \Gamma_{\theta\theta}^r &= -\frac{r}{h(r)}, & \Gamma_{\phi\phi}^r &= -\frac{r \sin^2\theta}{h(r)} \\ \Gamma_{tt}^r &= \frac{1}{2h(r)} \frac{df}{dr}, & \Gamma_{r\theta}^{\theta} &= \Gamma_{\theta r}^{\theta} = \frac{1}{r}, & \Gamma_{\phi\phi}^{\theta} &= -\sin\theta \cos\theta \\ \Gamma_{\phi r}^{\phi} &= \Gamma_{r\phi}^{\phi} = \frac{1}{r}, & \Gamma_{\phi\theta}^{\phi} &= \Gamma_{\theta\phi}^{\phi} = \cot\theta, & \Gamma_{rr}^t &= \Gamma_{rt}^t = \frac{1}{2f(r)} \frac{df}{dr} \end{aligned}$$

The Ricci tensor is found from:

$$R_{\mu\nu} = \frac{\partial \Gamma_{\mu\lambda}^{\lambda}}{\partial x^{\nu}} - \frac{\partial \Gamma_{\mu\nu}^{\lambda}}{\partial x^{\lambda}} - \Gamma_{\mu\lambda}^{\eta} \Gamma_{\eta\nu}^{\lambda} + \Gamma_{\mu\nu}^{\eta} \Gamma_{\eta\lambda}^{\lambda}$$

Show (ex.) $R_{\mu\nu} = 0$ for $\mu \neq \nu$

$$R_{rr} = - \left(\frac{f''(r)}{2f(r)} - \frac{1}{4} \left(\frac{f'(r)}{f(r)} \right) \left(\frac{h'(r)}{h(r)} + \frac{f'(r)}{f(r)} \right) - \frac{1}{r} \left(\frac{h'(r)}{h(r)} \right) \right)$$

$$R_{\theta\theta} = - \left(-1 + \frac{r}{2h(r)} \left(-\frac{h'(r)}{h(r)} + \frac{f'(r)}{f(r)} \right) + \frac{1}{h(r)} \right)$$

$$R_{\phi\phi} = \sin^2\theta R_{\theta\theta}$$

$$R_{tr} = - \left(-\frac{f''(r)}{2h(r)} + \frac{1}{4} \left(\frac{f'(r)}{f(r)} \right) \left(\frac{h'(r)}{h(r)} + \frac{f'(r)}{f(r)} \right) - \frac{1}{r} \left(\frac{f'(r)}{h(r)} \right) \right)$$



Thus for exterior solution we use vacuum Einstein's field equations.

Recall from lecture 13 the "trace-reversed" form

$$R_{\mu\nu} = 8\pi (T_{\mu\nu} - \frac{1}{2} T g_{\mu\nu})$$

which, in vacuum $T_{\mu\nu} = 0$ & $T = 0$:

$$R_{\mu\nu} = 0$$

It suffices to set just $R_{tt}, R_{rr}, R_{\theta\theta} = 0$

Note that:

$$\frac{R_{tt}}{f(r)} + \frac{R_{rr}}{h(r)} = -\frac{1}{r h(r)} \left(\frac{h'(r)}{h(r)} + \frac{f'(r)}{f(r)} \right) = 0$$

is

$$\frac{f'}{f} + \frac{h'}{h} = 0$$

or

$$f = k h^{-1}$$

Where k is a constant. By rescaling time
 $t \mapsto \sqrt{k} t$ we may set $k=1$

Equation $R_{\theta\theta} = 0$ then implies (ex):

$$-f' + \frac{1-f}{r} = 0$$

So that

$$\frac{d}{dr}(rf) = 1$$

That is

$$f = 1 + \frac{C}{r}$$

where C is a constant.

We have thus solved for the metric:

$$(*) \quad ds^2 = -\left(1 + \frac{C}{r}\right) dt^2 + \left(1 + \frac{C}{r}\right)^{-1} dr^2 + r^2 d\Omega^2$$

where $d\Omega^2 = d\theta^2 + \sin^2\theta d\phi^2$

This is the Schwarzschild metric (1916)

As $r \rightarrow \infty$ the metric approaches the Minkowski metric. To interpret constant we consider the behaviour of test body and compare with that of Newtonian theory (in weak-field limit).

Exercise: (*) suggests

$$C = -2m$$

Thus Schwarzschild metric becomes

$$ds^2 = - \left(1 - \frac{2M}{r} \right) dt^2 + \left(1 - \frac{2M}{r} \right)^{-1} dr^2 + r^2 d\Omega^2$$

There are two singularities, one at

$$r = 0 \quad \text{and one at} \quad r = 2m$$

The singularity at $r_s = 2m$ is a coordinate singularity (coordinate system breaks down; we won't argue this here.)

For "usual" objects (e.g. not Black holes) $r = 2m$ lies deep within the object. Eg. for the sun

$$r_s \approx 2.95 \text{ km}$$

where vacuum Einstein's equations do not apply